src/ManCompSoundness_Appraisal.v
@@ -2,57 +2,57 @@
       Namely, that the compiler outputs a collection of manifests that support 
       appraisal execution over the input evidence.  *)
 
-Require Import Manifest Manifest_Compiler Manifest_Generator ID_Type
+Require Import Manifest Attestation_Session Session_Config_Compiler Manifest_Generator ID_Type
   Maps Term_Defs List Cvm_St Cvm_Impl ErrorStMonad_Coq StructTactics 
   Cvm_Monad EqClass Manifest_Admits Auto.
 Require Import Manifest_Generator_Facts Eqb_Evidence ManCompSoundness.
+Require Import Manifest_Generator_Union.
 
 Require Import Coq.Program.Tactics Lia.
 
 Import ListNotations.
 
-Fixpoint am_config_support_exec_app (e : Evidence) (ac : AM_Config) : Prop :=
-    match e with
-    | mt => True 
-    | nn _ => True (* TODO: how to account for nonce handling? *)
-    | uu p fwd ps e' => 
-        let need_appr_asp :=
-          let '(asp_paramsC att_id arg targ targ_id) := ps in
-          match map_get (ASP_to_APPR_ASP_Map ac) att_id with
-          | Some appr_asp => 
-            (forall rawEv, 
-            (exists res, ac.(aspCb) (asp_paramsC appr_asp arg targ targ_id) rawEv = resultC res)
-            \/
-            (exists errStr, ac.(aspCb) (asp_paramsC appr_asp arg targ targ_id) rawEv = errC (Runtime errStr))
-            )
-          | None => False
-          end
-        in
-        match fwd with 
-        | ENCR => 
-            match ps with 
-            | asp_paramsC _ _ p _ => 
-                ((exists res, 
-                  ac.(pubKeyCb) p = resultC res) \/ 
-                (exists errStr, ac.(pubKeyCb) p = errC (Runtime errStr))) /\ 
-                am_config_support_exec_app e' ac /\
-                need_appr_asp
-            end
-        | (EXTD n) => 
-            am_config_support_exec_app e' ac /\
-            need_appr_asp
-        | KEEP => 
-            am_config_support_exec_app e' ac /\
-            need_appr_asp
-        | _ => True
+Fixpoint session_config_support_exec_app (e : Evidence) 
+    (sc : Session_Config) : Prop :=
+  match e with
+  | mt => True 
+  | nn _ => True (* TODO: how to account for nonce handling? *)
+  | uu p fwd ps e' => 
+      let need_appr_asp :=
+        let '(asp_paramsC att_id arg targ targ_id) := ps in
+        match map_get (ASP_to_APPR_ASP_Map sc) att_id with
+        | Some appr_asp => 
+          (forall rawEv, 
+          (exists res, sc.(aspCb) (asp_paramsC appr_asp arg targ targ_id) rawEv = resultC res)
+          \/
+          (exists errStr, sc.(aspCb) (asp_paramsC appr_asp arg targ targ_id) rawEv = errC (Runtime errStr))
+          )
+        | None => False
         end
-    | ss e1 e2 => 
-        exists ac1 ac2, 
-        (am_config_support_exec_app e1 ac1) /\ 
-        (am_config_support_exec_app e2 ac1) /\ 
-        supports_am ac1 ac /\
-        supports_am ac2 ac
-    end.
+      in
+      match fwd with 
+      | ENCR => 
+          match ps with 
+          | asp_paramsC _ _ p _ => 
+              (exists v, map_get (pubkey_map sc) p = Some v) /\
+              session_config_support_exec_app e' sc /\
+              need_appr_asp
+          end
+      | (EXTD n) => 
+          session_config_support_exec_app e' sc /\
+          need_appr_asp
+      | KEEP => 
+          session_config_support_exec_app e' sc /\
+          need_appr_asp
+      | _ => True
+      end
+  | ss e1 e2 => 
+      exists sc1 sc2, 
+      (session_config_support_exec_app e1 sc1) /\ 
+      (session_config_support_exec_app e2 sc1) /\ 
+      session_config_subset sc1 sc /\
+      session_config_subset sc2 sc
+  end.
 
 Require Import AM_St Impl_appraisal.
 
@@ -263,11 +263,11 @@ Proof.
     repeat find_eapply_hyp_hyp; subst; eauto.
 Qed.
 
-Theorem well_formed_am_config_impl_executable_app : forall et amConf ls,
-  am_config_support_exec_app et amConf ->
+Theorem well_formed_am_config_impl_executable_app : forall et sc ls,
+  session_config_support_exec_app et sc ->
   et_size et = length ls -> 
   forall st,
-  supports_am amConf (st.(amConfig)) ->
+  session_config_subset sc (st.(am_config)) ->
   has_nonces (nonce_ids_et et) (st.(am_nonceMap)) -> 
     (exists ec st',
         (gen_appraise_AM et ls) st = (resultC ec, st')) \/ 
@@ -318,30 +318,29 @@ Proof.
     unfold decrypt_bs_to_rawev' in *;
     monad_unfold; repeat ff; eauto;
     unfold am_failm, check_et_size, check_asp_EXTD in *;
-    simpl in *;
-    try match goal with
-    | H : forall _ : RawEv, _ \/ _,
-      H' : aspCb _ _ ?rawev = _ |- _ => 
-      let H'' := fresh "H" in
-      let H''' := fresh "H" in
-      let res := fresh "res" in
-      destruct (H rawev) as [H'' | H''];
-      destruct H'' as [res H''']; eauto
-    end; ff;
-    simpl in *; repeat find_injection; eauto;
-    unfold supports_am in *; intuition;
-    repeat (find_eapply_hyp_hyp; try find_rewrite; try find_injection);
-    try congruence; eauto;
+    repeat find_injection; repeat find_rewrite; eauto; try congruence;
     try (find_apply_lem_hyp decrypt_prim_runtime; subst; eauto; congruence); eauto.
-    * rewrite PeanoNat.Nat.eqb_eq in *;
+    * unfold session_config_subset in *; intuition;
+      repeat (find_eapply_hyp_hyp; try find_rewrite; try find_injection);
+      try congruence; eauto. 
+    * ff; repeat find_injection; eauto; congruence. 
+    * ff; repeat find_injection; eauto;
+      rewrite PeanoNat.Nat.eqb_eq in *; eauto;
+      subst; repeat find_rewrite; simpl in *;
       edestruct IHet; intuition; eauto;
       break_exists; find_rewrite; repeat find_injection;
       eauto; congruence.
-    * find_rewrite; find_injection; eauto.
+    * unfold session_config_subset in H1; intuition;
+      repeat find_apply_hyp_hyp;
+      repeat find_rewrite; repeat find_injection.
+      edestruct (H4 (r0 ++ r1)); break_exists; 
+      repeat find_rewrite; repeat find_injection; eauto;
+      find_apply_hyp_hyp; repeat find_rewrite;
+      repeat find_injection; try congruence; eauto.
     * edestruct IHet with (ls := r1); intuition; eauto;
-      break_exists; find_rewrite; repeat find_injection;
-      eauto; try congruence.
-      find_eapply_lem_hyp peel_n_am_res_spec; intuition; subst.
+      break_exists; repeat find_rewrite; repeat find_injection;
+      eauto; try congruence;
+      find_eapply_lem_hyp peel_n_am_res_spec; intuition; subst;
       rewrite app_length in *; lia.
   - (* ss case *)
     cbn in *.
@@ -350,7 +349,7 @@ Proof.
     edestruct IHet1 with (ls := firstn (et_size et1) ls).
     eassumption.
     2: {
-      eapply supports_am_trans; eauto.
+      eapply session_config_subset_trans; eauto.
     }
     2: {
       unfold nonce_ids_et.
@@ -385,7 +384,7 @@ Proof.
     eassumption.
 
     2: {
-      unfold supports_am in *.
+      unfold session_config_subset in *;
       destruct_conjs; repeat ff; intuition; eauto.
     }
 
@@ -464,16 +463,15 @@ Proof.
       eauto.
 Qed.
 
-Fixpoint manifest_support_term_app (m : Manifest) (al : AM_Library) (e : Evidence) : Prop :=
+Fixpoint manifest_support_term_app (m : Manifest) (e : Evidence) : Prop :=
     match e with
     | mt => True 
     | nn _ => True (* TODO: should we account for nonce presence here? *)
     | uu p fwd ps e' => 
         let appr_asp_sup :=
           let '(asp_paramsC att_id arg targ targ_id) := ps in
-          match map_get (ASP_Compat_Map al) att_id with
-          | Some appr_asp => 
-            In_set appr_asp m.(asps)
+          match map_get (ASP_Compat_Map m) att_id with
+          | Some appr_asp => In_set appr_asp m.(asps)
           | None => False
           end
         in
@@ -481,77 +479,109 @@ Fixpoint manifest_support_term_app (m : Manifest) (al : AM_Library) (e : Evidenc
         | (EXTD n) => 
           match ps with 
           | asp_paramsC a _ targ  _ => 
-              manifest_support_term_app m al e' /\
+              manifest_support_term_app m e' /\
               appr_asp_sup
           end
         | ENCR => 
         match ps with 
         | asp_paramsC _ _ p _ =>
-            In_set p m.(pubKeyPlcs) /\ 
-            manifest_support_term_app m al e' /\
+            manifest_support_term_app m e' /\
             appr_asp_sup
         end
 
         | KEEP => 
-            manifest_support_term_app m al e' /\
+            manifest_support_term_app m e' /\
             appr_asp_sup
 
         | _ => True
         end
         (* TODO:  support other fwd types here in the future... *)
     | ss e1 e2 => 
-        manifest_support_term_app m al e1 /\ 
-        manifest_support_term_app m al e2
+        manifest_support_term_app m e1 /\ 
+        manifest_support_term_app m e2
     end.
 
-Definition lib_config_compatible (al : AM_Library) (ac : AM_Config) : Prop :=
-  forall a0 a',
-    map_get (ASP_Compat_Map al) a0 = Some a' ->
-    map_get (ASP_to_APPR_ASP_Map ac) a0 = Some a'.
+Fixpoint att_sess_supports_term_app (ats : Attestation_Session) (e : Evidence) 
+    : Prop :=
+  match e with
+  | mt => True 
+  | nn _ => True (* TODO: should we account for nonce presence here? *)
+  | uu p fwd ps e' => 
+      match fwd with 
+      | (EXTD n) => 
+          match ps with 
+          | asp_paramsC a _ targ  _ => 
+              att_sess_supports_term_app ats e'
+          end
+      | ENCR => 
+          match ps with 
+          | asp_paramsC _ _ p _ =>
+              att_sess_supports_term_app ats e' /\
+              (exists v, map_get (PubKey_Mapping ats) p = Some v)
+          end
+      | KEEP => 
+          att_sess_supports_term_app ats e'
+      | _ => True
+      end
+      (* TODO:  supports other fwd types here in the future... *)
+  | ss e1 e2 => 
+      att_sess_supports_term_app ats e1 /\ 
+      att_sess_supports_term_app ats e2
+  end.
 
-Theorem manifest_support_am_config_impl_am_config_app: forall et absMan amConf al,
-    manifest_support_am_config absMan amConf ->
-    lib_config_compatible al amConf ->
-    manifest_support_term_app absMan al et ->
-    am_config_support_exec_app et amConf.
+Require Import AM_Manager.
+
+Theorem manifest_support_sc_impl_sc_exec: forall t absMan ats,
+  well_formed_manifest absMan ->
+  manifest_support_term_app absMan t ->
+  att_sess_supports_term_app ats t ->
+  forall aspBin uuid,
+  session_config_support_exec_app
+    t 
+    (session_config_compiler (mkAM_Man_Conf absMan aspBin uuid) ats).
 Proof.
-  induction et; simpl in *; intuition; eauto;
-  unfold manifest_support_am_config in *; intuition; eauto.
-  - repeat (try break_match; simpl in *; intuition; eauto);
-    unfold lib_config_compatible in *; intuition; 
-    repeat (find_eapply_hyp_hyp; try find_rewrite; try find_injection);
-    simpl in *; intuition; eauto; try congruence.
-  - repeat (try break_match; simpl in *; intuition; eauto).  
-    pose proof (IHet1 absMan amConf al); 
-      pose proof (IHet2 absMan amConf); intuition.
-      repeat eexists; eauto.
-  Unshelve.
-  all: eauto.
-  all: eapply nil.
+  induction t; simpl in *; intuition; eauto.
+  - repeat (break_match; simpl in *; intuition; eauto);
+    unfold well_formed_manifest in *; find_apply_hyp_hyp;
+    break_exists; repeat find_rewrite; repeat find_injection;
+    eauto; try congruence.
+  - repeat eexists; eauto.
 Qed.
 
-Lemma manifest_supports_term_sub_app : forall m1 m2 et al,
+Lemma manifest_supports_term_sub_app : forall m1 m2,
   manifest_subset m1 m2 ->
-  manifest_support_term_app m1 al et -> 
-  manifest_support_term_app m2 al et.
+  (forall k v, 
+    map_get (ASP_Compat_Map m1) k = Some v ->
+    map_get (ASP_Compat_Map m2) k = Some v
+  ) ->
+  forall et,
+  manifest_support_term_app m1 et -> 
+  manifest_support_term_app m2 et.
 Proof.
-  intros.
-  generalizeEverythingElse et.
-  induction et; intros; ff.
+  intros m1 m2 HS HCM.
+  induction et; intuition; simpl in *; eauto.
   - (* asp case *)
-    subst.
-    unfold manifest_subset in H. 
-    destruct_conjs.
-    ff; subst; intuition; eauto;
-    eapply IHet; eauto; unfold manifest_subset; eauto.
-  -
-    split; 
-    destruct_conjs; ff; eauto.
+    repeat (break_match; simpl in *; subst; 
+      repeat find_apply_hyp_hyp;
+      repeat find_rewrite; repeat find_injection;
+      intuition; eauto; try congruence).
+  - intuition.
 Qed.
 
-Lemma manifest_generator_app_cumul : forall et m1 m1' m2 al,
+Lemma manifest_subset_aspid_update : forall m1 m2 a,
   manifest_subset m1 m2 ->
-  manifest_generator_app'' et al m2 = resultC m1' ->
+  manifest_subset m1 (aspid_manifest_update a m2).
+Proof.
+  intuition; unfold manifest_subset in *; intuition;
+  find_apply_hyp_hyp; unfold aspid_manifest_update;
+  destruct m2; simpl in *; 
+  pose proof @in_set_add; eauto.
+Qed.
+Global Hint Resolve manifest_subset_aspid_update : core.
+
+Lemma manifest_generator_app_cumul : forall et m1 m1' m2 cm,
+  manifest_subset m1 m2 ->
+  manifest_generator_app' cm et m2 = resultC m1' ->
   manifest_subset m1 m1'.
 Proof.
   intros.
@@ -559,58 +589,12 @@ Proof.
   induction et; intros; ff; eauto.
   - (* uu case *)
     subst; ff; eauto.
-    + (* ENCR *)
-
-    subst.
-
-    unfold pubkey_manifest_update in *.
-    break_let.
-    subst.
-    unfold manifest_subset in *.
-    simpl in *.
-    destruct_conjs.
-
-    edestruct IHet; eauto;
-    simpl in *; intuition; eauto;
-    find_apply_hyp_hyp; eauto.
-    * eapply H4; eauto;
-      eapply in_set_add; eauto.
-    * eapply H5; eauto;
-      eapply in_set_add; eauto.
-
-    + (* EXTD *)
-
-    unfold aspid_manifest_update in *.
-    break_let.
-    subst.
-    unfold manifest_subset in *.
-    simpl in *.
-    destruct_conjs.
-
-    edestruct IHet; intuition; eauto;
-    simpl in *.
-    find_apply_hyp_hyp; eauto.
-    eapply H4.
-    eapply in_set_add; eauto.
-    + subst; unfold aspid_manifest_update in *;
-    break_let.
-    subst.
-    unfold manifest_subset in *.
-    simpl in *.
-    destruct_conjs.
-
-    edestruct IHet; eauto;
-    simpl in *; intuition; eauto;
-    find_apply_hyp_hyp; eauto.
-    eapply H4; eauto.
-    eapply in_set_add; eauto.
-    
   - (* ss case *)
     ff; eauto.
 Qed.
 
-Lemma manifest_generator_app_cumul' : forall et m1 al m1',
-  manifest_generator_app'' et al m1 = resultC m1' ->
+Lemma manifest_generator_app_cumul' : forall et m1 cm m1',
+  manifest_generator_app' cm et m1 = resultC m1' ->
   manifest_subset m1 m1'.
 Proof.
   intros.
@@ -619,53 +603,74 @@ Proof.
   eauto.
 Qed.
 
-
-Lemma asdf_app : forall et1 et2 absMan m m' al,
-  manifest_generator_app'' et1 al m = resultC m' ->
-  manifest_generator_app'' et2 al m' = resultC absMan ->
+Lemma asdf_app : forall et1 et2 absMan m m' cm,
+  manifest_generator_app' cm et1 m = resultC m' ->
+  manifest_generator_app' cm et2 m' = resultC absMan ->
   exists m'',
-  manifest_generator_app'' et1 al m = resultC m'' /\ 
+  manifest_generator_app' cm et1 m = resultC m'' /\ 
   manifest_subset m'' absMan.
-  Proof.
-    intros.
-    eexists.
-    split; try reflexivity.
-    rewrite <- H; eauto.
-    eapply manifest_generator_app_cumul'; eauto.
+Proof.
+  intros.
+  eexists.
+  split; try reflexivity.
+  rewrite <- H; eauto.
+  eapply manifest_generator_app_cumul'; eauto.
 Qed.
 
-Theorem man_gen_old_always_supports_app : forall et oldMan absMan al,
-  manifest_generator_app'' et al oldMan = resultC absMan ->
-  manifest_support_term_app absMan al et.
+Lemma compat_map_never_change_mangen_app : forall cm et oldMan absMan, 
+  manifest_generator_app' cm et oldMan = resultC absMan ->
+  (ASP_Compat_Map oldMan) = (ASP_Compat_Map absMan).
+Proof.
+  induction et; simpl in *; intuition; 
+  repeat find_rewrite; repeat find_injection; eauto.
+  - ff; find_apply_hyp_hyp; unfold aspid_manifest_update in *;
+    destruct oldMan; simpl in *; intuition; eauto.
+  - ff; eapply IHet1 in Heqr;
+    eapply IHet2 in H; repeat find_rewrite; eauto.
+Qed.
+
+Theorem man_gen_old_always_supports_app : forall et oldMan absMan cm,
+  (* (forall k v, 
+    map_get cm k = Some v ->
+    map_get (ASP_Compat_Map absMan) k = Some v
+  ) -> *)
+  manifest_generator_app' cm et oldMan = resultC absMan ->
+  manifest_support_term_app (add_compat_map_manifest absMan cm) et.
 Proof.
   induction et; intuition;
     repeat (try break_match; 
-      unfold app_aspid_manifest_update in *;
-      (*
-      unfold manifest_generator_app' in *;
-      unfold manifest_generator_app'' in *; *)
-      unfold aspid_manifest_update, pubkey_manifest_update in *;
+      unfold aspid_manifest_update in *;
       subst; simpl in *; intuition; eauto; try congruence;
       repeat find_rewrite;
       repeat find_injection;
       simpl in * );
     try (rewrite mapC_get_works in *; simpl in *; repeat find_injection; simpl in *; intuition; eauto; congruence); 
     repeat (ff; simpl in *; subst; intuition; eauto);
-  match goal with
-  | H : manifest_generator_app'' _ _ ?m' = resultC ?m |- _ =>
-      assert (manifest_subset m' m) by (eapply manifest_generator_app_cumul'; eauto);
-      unfold manifest_subset in *;
-      intuition; simpl in *; eauto
-  end.
-  - eapply H2; simpl in *.
-    unfold pubkey_manifest_update;
-    ff; eauto;
-    eapply manadd_In_add.
-  - repeat find_eapply_hyp_hyp.
-    eapply manifest_supports_term_sub_app; eauto;
-    unfold manifest_subset; intuition.
+  try (find_apply_lem_hyp manifest_generator_app_cumul';
+    unfold manifest_subset in *; simpl in *;
+    pose proof @manadd_In_add; eauto;
+    unfold add_compat_map_manifest in *;
+    destruct absMan; simpl in *; intuition; eauto;
+    repeat find_rewrite; repeat find_injection;
+    eauto; congruence).
+  - 
+    pose proof (compat_map_never_change_mangen_app _ _ _ _ Heqr);
+    pose proof (compat_map_never_change_mangen_app _ _ _ _ H);
+    repeat find_rewrite;
+    pose proof (asdf_app _ _ _ _ _ _ Heqr H);
+    break_exists; intuition;
+    repeat find_rewrite; repeat find_injection.
+    eapply IHet2 in H; eauto;
+    eapply IHet1 in Heqr; eauto; repeat find_rewrite; eauto.
+    clear IHet1 IHet2.
+    eapply manifest_supports_term_sub_app in Heqr.
+    * eauto. 
+    * destruct x, absMan; simpl in *;
+      intuition.
+    * destruct x, absMan; simpl in *; eauto.
 Qed.
 
+(*
 Lemma lib_config_compatible_man_comp : forall al aspBin absMan,
   lib_config_compatible al (manifest_compiler absMan al aspBin).
 Proof.
@@ -696,7 +701,7 @@ Theorem manifest_generator_compiler_soundness_app : forall et ls oldMan absMan a
     ).
 Proof.
   intros.
-  assert (supports_am amConf (st.(amConfig))) by (find_rewrite; eauto using supports_am_refl).
+  assert (session_config_subset amConf (st.(amConfig))) by (find_rewrite; eauto using session_config_subset_refl).
 
   eapply well_formed_am_config_impl_executable_app.
   - unfold manifest_generator, e_empty in *; simpl in *.
@@ -748,11 +753,12 @@ Proof.
     eauto.
 Qed.
 Global Hint Resolve mangen_plcTerm_list_exists : core.
+*)
 
-Lemma mangen_plcEvidence_list_spec : forall ls et tp env envL al,
+Lemma mangen_plcEvidence_list_spec : forall ls et tp env envL cm,
   In (et, tp) ls ->
-  manifest_generator_plcEvidence_list ls al = resultC envL ->
-  manifest_generator_app et tp al = resultC env ->
+  manifest_generator_plcEvidence_list cm ls = resultC envL ->
+  manifest_generator_app cm et tp = resultC env ->
   In env envL.
 Proof.
   induction ls; simpl in *; intuition; subst; eauto;
@@ -763,13 +769,13 @@ Proof.
 Qed.
 Global Hint Resolve mangen_plcTerm_list_spec : core.
 
-Lemma mangen_plcEvidence_list_subsumes : forall ls p m envL al,
-  mangen_plcEvidence_list_union ls al = resultC envL ->
+Lemma mangen_plcEvidence_list_subsumes : forall ls p m envL cm,
+  mangen_plcEvidence_list_union cm ls = resultC envL ->
   map_get envL p = Some m ->
   (forall et tp,
     In (et,tp) ls ->
     (forall env' m', 
-      manifest_generator_app et tp al = resultC env' ->
+      manifest_generator_app cm et tp = resultC env' ->
       map_get env' p = Some m' ->
       manifest_subset m' m
     )
@@ -783,21 +789,20 @@ Qed.
 Global Hint Resolve mangen_plcTerm_list_subsumes : core.
 
 
-Lemma mangen_plcEvidence_subset_end_to_end_mangen : forall ls et tp al,
+Lemma mangen_plcEvidence_subset_end_to_end_mangen : forall ls et tp cm,
   In (et, tp) ls ->
   (forall m m' p,
     forall envL, 
-      mangen_plcEvidence_list_union ls al = resultC envL ->
+      mangen_plcEvidence_list_union cm ls = resultC envL ->
       map_get envL p = Some m' ->
       forall ts envL', 
-        end_to_end_mangen' ls ts al = resultC envL' ->
+        end_to_end_mangen cm ls ts = resultC envL' ->
         map_get envL' p = Some m ->
         manifest_subset m' m
   ).
 Proof.
-  intuition; unfold end_to_end_mangen' in *.
+  intuition; unfold end_to_end_mangen in *.
   ff.
-  pose proof (manifest_env_union_always_subset).
   find_eapply_lem_hyp manifest_env_union_always_subset.
   intuition.
 Qed.
@@ -805,16 +810,16 @@ Global Hint Resolve mangen_plcTerm_subset_end_to_end_mangen : core.
 
 Lemma mangen_subset_end_to_end_mangen_app : forall ls et tp,
   In (et, tp) ls ->
-  (forall m m' p al env,
-    manifest_generator_app et tp al = resultC env ->
+  (forall m m' p cm env,
+    manifest_generator_app cm et tp = resultC env ->
     map_get env p = Some m' ->
     forall ts env', 
-      end_to_end_mangen' ls ts al = resultC env' ->
+      end_to_end_mangen cm ls ts = resultC env' ->
       map_get env' p = Some m ->
       manifest_subset m' m
   ).
 Proof.
-  intuition; unfold end_to_end_mangen' in *; ff.
+  intuition; unfold end_to_end_mangen in *; ff.
   find_eapply_lem_hyp manifest_env_union_always_subset; intuition.
   unfold mangen_plcEvidence_list_union in *.
   ff.
@@ -864,8 +869,8 @@ Global Hint Resolve mangen_exists_end_to_end_mangen_app : core.
 *)
 
 Lemma mangen_exists_end_to_end_mangen_app :
-  (forall et tp al env,
-    manifest_generator_app et tp al = resultC env ->
+  (forall et tp cm env,
+    manifest_generator_app cm et tp = resultC env ->
     exists m', map_get env tp = Some m'
   ).
 Proof.
@@ -882,16 +887,14 @@ Proof.
 Qed.
 Global Hint Resolve mangen_exists_end_to_end_mangen_app : core.
 
-
-
-Lemma mangen_app_tp_get : forall et tp x al env,
-  manifest_generator_app et tp al = resultC env ->
+(* 
+Lemma mangen_app_tp_get : forall et tp x cm env,
+  manifest_generator_app cm et tp = resultC env ->
   map_get env tp = Some x ->
-  manifest_generator_app'' et al (myPlc_manifest_update tp empty_Manifest) = resultC x.
+  manifest_generator_app' cm et x' = resultC x.
 Proof.
   intros.
   unfold manifest_generator_app in *.
-  unfold manifest_generator_app' in *.
   unfold manifest_update_env_res in *.
   unfold e_empty in *.
   ff.
@@ -900,51 +903,204 @@ Proof.
     rewrite String.eqb_eq.
     trivial.
   }
-  repeat find_rewrite.
+  repeat find_rewrite;
+  repeat find_injection.
   ff.
 Qed.
+*)
+(* Lemma end_to_end_mangen_all_same_cm : forall cm ls ts env,
+  end_to_end_mangen cm ls ts = resultC env ->
+  (forall p m,
+    map_get env p = Some m ->
+    cm = m.(ASP_Compat_Map)
+  ).
+Proof.
+  intuition.
+  unfold end_to_end_mangen in *; ff.
+  unfold mangen_plcEvidence_list_union,
+    manifest_generator_plcEvidence_list,
+    mangen_plcTerm_list_union,
+    manifest_generator_plcTerm_list in *; ff.
+  eapply manifest_env_union_map_one_fwd in H0;
+  break_exists; intuition; eauto.
+  Search (map_get (Manifest_Union.environment_union _ _) _ = _). *)
+  
+Lemma mangen_app_same_comp_map : forall et tp cm env,
+  manifest_generator_app cm et tp = resultC env ->
+  forall k v,
+    map_get env k = Some v ->
+    cm = (ASP_Compat_Map v).
+Proof.
+  intros.
+  unfold manifest_generator_app,
+    res_bind, manifest_update_env_res in *;
+  repeat ff.
+  unfold add_compat_map_manifest; 
+  destruct m; simpl in *; eauto.
+Qed.
 
-Lemma end_to_end_mangen_supports_all_app : forall ts ls tp m env al,
-  end_to_end_mangen' ls ts al = resultC env ->
+Lemma map_get_under_invariant : forall P m1 m2,
+  (forall k v, map_get m1 k = Some v -> P v) ->
+  (forall k v, map_get m2 k = Some v -> P v) ->
+  (forall v1 v2, P v1 -> P v2 -> P (Manifest_Union.manifest_union_asps v1 v2)) ->
+  (forall k v, map_get (Manifest_Union.environment_union m1 m2) k = Some v -> P v).
+Proof.
+  intuition.
+  eapply manifest_env_union_works in H.
+  Search (map_get (Manifest_Union.environment_union _ _) _ = _).
+
+  (forall k v, map_get m k = Some v -> P k v) ->
+  P k v.
+ 
+Lemma end_to_end_mangen_same_comp_map : forall et tp cm env,
+  end_to_end_mangen cm et tp = resultC env ->
+  forall k v,
+    map_get env k = Some v ->
+    cm = (ASP_Compat_Map v).
+Proof.
+  intros.
+  unfold end_to_end_mangen,
+    res_bind, manifest_update_env_res in *;
+  repeat ff.
+  assert (forall k v', 
+    map_get (Maps.map_map (fun m : Manifest =>
+    add_compat_map_manifest m cm) 
+    (mangen_plcTerm_list_union tp)) k = Some v' ->
+    cm = ASP_Compat_Map v'). {
+      clear H0 Heqr.
+      induction (mangen_plcTerm_list_union tp);
+      simpl in *; intuition; eauto; try congruence;
+      simpl in *; ff; eauto;
+      destruct b; simpl in *; eauto.
+  }
+  assert (forall k v', 
+    map_get e k = Some v' ->
+    cm = ASP_Compat_Map v'). {
+      clear H H0.
+      unfold mangen_plcEvidence_list_union,
+        manifest_generator_plcEvidence_list in *;
+      ff; intuition.
+      generalize dependent l.
+      induction et; simpl in *; intuition; 
+      repeat find_rewrite; ff; try congruence.
+      unfold res_bind in *; ff; eauto.
+
+
+      Search (result_map).
+      eapply result_map_spec in Heqr0.
+      * break_exists; intuition. 
+        Search manifest_generator_app.
+
+      induction l; simpl in *; intuition; try congruence;
+      eauto.
+      eapply result_map_spec in Heqr0.
+      induction (mangen_plcTerm_list_union tp);
+      simpl in *; intuition; eauto; try congruence;
+      simpl in *; ff; eauto;
+      destruct b; simpl in *; eauto.
+  }
+  Search (map_get (Manifest_Union.environment_union _ _) _ = _).
+  eapply manifest_env_union_map_one_fwd in H0;
+  break_exists; intuition.
+  - admit. 
+  -  
+  unfold add_compat_map_manifest in *.
+  
+  destruct m; simpl in *; eauto.
+Qed.
+
+(* Lemma add_compat_map_manifest_same : forall m x,
+  add_compat_map_manifest x (ASP_Compat_Map m) = m ->
+  (ASP_Compat_Map x) = (ASP_Compat_Map m).
+Proof.
+  destruct x; simpl in *; intuition; repeat find_injection; eauto.
+Qed. *)
+
+Lemma end_to_end_mangen_supports_all_app : forall ts ls tp m env cm,
+  end_to_end_mangen cm ls ts = resultC env ->
   map_get env tp = Some m ->
   (forall et, 
     In (et, tp) ls ->
-    (* In p (places tp t) -> *)
-    ((* forall t',
-      In t' (place_terms t tp p) -> *)
-      manifest_support_term_app m al et
-    )
+    manifest_support_term_app m et
   ).
 Proof.
   intuition.
   
-  destruct (manifest_generator_app et tp al) eqn:E.
-  - unfold end_to_end_mangen' in *; ff.
+  destruct (manifest_generator_app cm et tp) eqn:E.
+  - unfold end_to_end_mangen in *; ff.
     unfold mangen_plcEvidence_list_union in *; ff.
     unfold manifest_generator_plcEvidence_list in *; ff.
     pose proof (result_map_spec _ _ _ _ H1 Heqr0);
     break_exists; intuition; congruence.
-  - pose proof (mangen_exists_end_to_end_mangen_app et tp al _ E).
+  - pose proof (mangen_exists_end_to_end_mangen_app et tp _ _ E).
     break_exists.
     pose proof (mangen_subset_end_to_end_mangen_app _ _ _ H1 _ _ _ _ _ E H2 _ _ H H0). 
+    pose proof (mangen_app_same_comp_map _ _ _ _ E _ _ H2).
+    unfold manifest_generator_app,
+      res_bind, manifest_update_env_res in *;
+    repeat ff.
+    eapply man_gen_old_always_supports_app in Heqr0.
+    find_rewrite.
     eapply manifest_supports_term_sub_app; eauto.
-    eapply man_gen_old_always_supports_app.
-    eapply mangen_app_tp_get; eauto.
+    eauto.
+    * admit. 
+    * eapply add_compat_map_manifest_same in H5.
+
+    assert (cm = (ASP_Compat_Map x)).
+    {
+      eapply compat_map_never_change_mangen_app; eauto.
+    }
+    Search manifest_support_term_app.
+    eapply manifest_supports_term_sub_app; eauto.
+    * admit.  
+    * unfold manifest_generator_app in *.
+      unfold manifest_update_env_res in *.
+      unfold e_empty in *.
+      ff.
+      subst.
+      assert (String.eqb tp tp = true).
+      {
+        rewrite String.eqb_eq.
+        trivial.
+      }
+      repeat find_rewrite;
+      repeat find_injection.
+      clear H4.
+      admit.
+Admitted.
+(* 
+      assert (cm = (ASP_Compat_Map x)). admit.
+      eapply man_gen_old_always_supports_app in Heqr.
+      **  eapply manifest_supports_term_sub_app.
+        3: {
+          eapply Heqr.
+        }
+      eauto.
+      pose proof (manifest_supports_term_sub_app).
+      rewrite <- H2 in *.
+      subst.
+      subst.
+      Search manifest_generator_app.
+      eapply E.
+      unfold manifest_generator_app in *.
+      ** admit.
+      ** unfold res_bind in *;
+        ff.
 Qed.
-Global Hint Resolve end_to_end_mangen_supports_all : core.
+Global Hint Resolve end_to_end_mangen_supports_all : core. *)
 
-
-
-Theorem manifest_generator_compiler_soundness_distributed_multiterm_app : forall et ts ls bs tp absMan amLib amConf aspBin env,
-  end_to_end_mangen' ls ts amLib = resultC env ->
+Theorem manifest_generator_compiler_soundness_distributed_multiterm_app : forall et ts ls bs tp absMan cm sc aspBin env att_sess uuid,
+  end_to_end_mangen cm ls ts = resultC env ->
   map_get env tp = Some absMan -> 
   In (et,tp) ls ->
-  lib_supports_manifest amLib absMan ->
-  manifest_compiler absMan amLib aspBin = amConf ->
+  well_formed_manifest absMan ->
+  att_sess_supports_term_app att_sess et ->
+  manifest_support_session_conf absMan sc ->
+  session_config_compiler (mkAM_Man_Conf absMan aspBin uuid) att_sess = sc ->
   et_size et = length bs ->
   forall st,
 
-  supports_am amConf st.(amConfig)  ->
+  session_config_subset sc st.(am_config)  ->
 
   has_nonces (nonce_ids_et et) (st.(am_nonceMap)) -> 
 
@@ -957,15 +1113,11 @@ Theorem manifest_generator_compiler_soundness_distributed_multiterm_app : forall
 Proof.
   intros.
   eapply well_formed_am_config_impl_executable_app.
-  - unfold manifest_generator, e_empty in *; simpl in *.
-    eapply manifest_support_am_config_impl_am_config_app.
-    * eapply manifest_support_am_config_compiler; eauto.
-    * eapply lib_config_compatible_man_comp.
-    * (* NOTE: This is the important one, substitute proof of any manifest here *)
-      eapply end_to_end_mangen_supports_all_app; eauto.
+  - eapply manifest_support_sc_impl_sc_exec; eauto.
+    eapply end_to_end_mangen_supports_all_app; eauto.
   - find_rewrite; eauto.
   - match goal with
-    | H: manifest_compiler _ _ _ = _ |- _ => rewrite H; eauto
+    | H: session_config_compiler _ _ = _ |- _ => rewrite H; eauto
     end.
   - eauto.
 Qed.
